\documentclass{article}
\usepackage{graphicx}
\usepackage{mathtools}
\usepackage{amsmath}
\usepackage{amsmath}
\usepackage[makeroom]{cancel}

\newcommand{\Mod}[1]{\ (\mathrm{mod}\ #1)}


\begin{document}	

\textbf{\textit{Dipshitmaths}}

\begin{flushright}
	O-LEVEL 
	
	MATHEMATICS
	
	PROBLEM SET-WEEK 0
\end{flushright}

\begin{enumerate}
	\item  Simplify $\frac{4p^2r}{3}\div\frac{2r^3}{p}$
	
	\[
		\frac{4p^2r}{3}\div\frac{2r^3}{p}
	\]
	\[
		= \frac{4p^2r}{3}\times\frac{p}{2r^3}
	\]
	\[
		= \frac{\cancel{4}2p^2\cancel{r}}{3}\times\frac{p}{\cancel{2}\cancel{r^3}r^2}
	\]
	\[
		= \frac{2p^3}{3r^2}
	\]
		
		
	\item $a=\frac{3b+4c}{5-b}$
		\begin{enumerate}
			\item Evaluate $a$ when $b=6$ and $c=-2$
			\[
				a = \frac{3b+4c}{5-b}
			\]
			\[
				= \frac{3(6)+4(-2)}{5-(6)}
			\]
			\[
				= \frac{18-8}{-1} 
			\]
			\[
				= -10
			\]
			
			\item Express $b$ in terms of $a$ and $c$
			\[
				a = \frac{3b+4c}{5-b}
			\]
			\[
				a(5-b) = 3b+4c
			\]
			\[
				5a-ab = 3b+4c
			\]
			\[
				5a-4c = 3b+ab
			\]
			\[
				5a-4c = b(3+a)
			\]
			\[
				b = \frac{a+3}{5a-4c}
			\]
		\end{enumerate}

	\item 
		\begin{enumerate}
			\item Express $9-7x+x^2$ in the form $p+(q+x)^2$
			
			\[
				p+(q+x)^2 = 9-7x+x^2
			\]
			\[
				p + (q+x)(q+x) = p + q^2 + 2qx + x^2 = 9-7x+x^2
			\]
			Solving for each terms,	
			\[
				2qx = -7x
			\]
			\[
				q = -7/2 = -3.5
			\]
			\[
				p + q^2 = 9
			\]
			\[
				p = 9 - q^2 = 9 - (3.5)^2 = 9 - 12.25 = -3.25
			\]
			
			
			\item Write down the coordinates of the minimum point of the graph of $9-7x+x^2$
			
			Minimum point occurs when first derivative/tangent of the graph equals to zero
			\[
				y = 9-7x+x^2
			\]
			\[
				\frac{dy}{dx} = -7 + 2x = 0			
			\]
			\[
				x = 3.5
			\]
			\[
				y = 9 - 7(3.5) + (3.5)^2 = 9 - 24.5 + 12.25 = -3.25
			\]
			
			
		\end{enumerate}
	
	\item Solve $\frac{1}{x-3} + \frac{6}{x-1} = 2$
	\[
		\frac{1}{x-3} + \frac{6}{x-1} 	
	\]
	\[
		= \frac{x-1}{(x-3)(x-1)} + \frac{6(x-3)}{(x-3)(x-1)}  
	\]
	\[
		= \frac{(x-1) + 6(x-3)}{(x-3)(x-1)} 
	\]
	\[
		= \frac{x-1+6x-18}{x^2-4x+3}
	\]
	\[
		= \frac{7x-19}{x^2-4x+3}
	\]
	We know that
	\[
		\frac{7x-19}{x^2-4x+3} = 2
	\]
	\[
		7x-19 = 2(x^2-4x+3) = 2x^2-8x+6
	\]
	\[
		0 = 2x^2-8x-7x+6+19 = 2x^2-15x+25
	\]
	Factorizing,
	\[
		2x^2-15x+21 = (2x-5)(x-5) = 0
	\]
	Thus we have two solutions $2x-5 = 0$ and $x-5=0$
	
	\[
		2x_1-5 = 0
	\]
	\[
		x_1 = 5/2 = 2.5
	\]
	\[
		x_2-5 = 0
	\]
	\[
		x_2 = 5
	\]
	
	
	
\end{enumerate}



\end{document}